introduce and prove invariant LearnedImpliesQuorumOfAcceptors

messageInvariantPrototypes/paxos/centralized/applicationProof.dfy
@@ -7,9 +7,44 @@ import opened UtilitiesLibrary
 import opened System
 import opened Obligations
 
+// Learner's receivedAccepts contain valid acceptor ids 
+ghost predicate LearnerValidReceivedAccepts(c: Constants, v: Variables)
+  requires v.WF(c)
+{
+  forall lnr:LearnerId, vb:ValBal, e:AcceptorId |
+    && c.ValidLearnerIdx(lnr)
+    && vb in v.learners[lnr].receivedAccepts
+    && e in v.learners[lnr].receivedAccepts[vb]
+  ::
+    c.ValidAcceptorIdx(e)
+}
+
+// Learner's learned value must be backed by a quorum of accepts
+ghost predicate LearnedImpliesQuorumOfAcceptors(c: Constants, v: Variables)
+  requires v.WF(c)
+{
+  forall lnr:LearnerId, val:Value |
+    && c.ValidLearnerIdx(lnr)
+    && v.learners[lnr].HasLearnedValue(val)
+  ::
+    exists b: LeaderId ::
+      && var vb := VB(val, b);
+      && vb in v.learners[lnr].receivedAccepts
+      && IsAcceptorQuorum(c, v.learners[lnr].receivedAccepts[vb])
+}
+
+// Application bundle
+ghost predicate ApplicationInv(c: Constants, v: Variables)
+  requires v.WF(c)
+{
+  && LearnerValidReceivedAccepts(c, v)
+  && LearnedImpliesQuorumOfAcceptors(c, v)
+}
+
 ghost predicate Inv(c: Constants, v: Variables)
 {
   && v.WF(c)
+  && ApplicationInv(c, v)
   && Agreement(c, v)
 }
 
@@ -34,7 +69,51 @@ lemma InvInductive(c: Constants, v: Variables, v': Variables)
   requires Next(c, v, v')
   ensures Inv(c, v')
 {
+  InvNextLearnedImpliesQuorumOfAcceptors(c, v, v');
+  assert ApplicationInv(c, v');
+
   // TODO
   assume false;
 }
+
+
+/***************************************************************************************
+*                                 InvNext Proofs                                       *
+***************************************************************************************/
+
+lemma InvNextLearnedImpliesQuorumOfAcceptors(c: Constants, v: Variables, v': Variables)
+  requires v.WF(c)
+  requires LearnerValidReceivedAccepts(c, v)
+  requires LearnedImpliesQuorumOfAcceptors(c, v)
+  requires Next(c, v, v')
+  ensures LearnedImpliesQuorumOfAcceptors(c, v')
+{
+  forall lnr:LearnerId, val:Value |
+    c.ValidLearnerIdx(lnr) && v'.learners[lnr].HasLearnedValue(val)
+  ensures
+    exists b: LeaderId ::
+      && var vb := VB(val, b);
+      && vb in v'.learners[lnr].receivedAccepts
+      && IsAcceptorQuorum(c, v'.learners[lnr].receivedAccepts[vb])
+  {
+    var sysStep :| NextStep(c, v, v', sysStep);
+    if sysStep.P2bStep? {
+      if sysStep.learner == lnr {
+        // trigger
+        assert v.learners[lnr].HasLearnedValue(val);
+      }
+    }
+  }
 }
+
+
+/***************************************************************************************
+*                            Helper Definitions and Lemmas                             *
+***************************************************************************************/
+
+ghost predicate IsAcceptorQuorum(c: Constants, quorum: set<AcceptorId>) {
+  && |quorum| >= c.f+1
+  && (forall id | id in quorum :: c.ValidAcceptorIdx(id))
+}
+
+} // end module PaxosProof
